iris/IntrDefs.v
@@ -531,6 +531,7 @@ Section IntrDefs.
         = Some (Supervisor, σ) ->
       exec (is_shadow_stack_access acc) σ = Some (false, σ) ->
       pma_allows_all (register_lookup pma_regions σ.(sregs)) ->
+      kadm_ident va ppn ->
       ↑kptN ⊆ E ->
       ⊢ kmap_at (svpn_of va) ppn pc -∗
         reg_interp σ.(sregs) -∗ gen_heap_interp σ.(mem) -∗ strans_inv ={E}=∗
@@ -543,15 +544,15 @@ Section IntrDefs.
           ⌜ pmp_grant_facts σ' ⌝ ∗
           reg_interp σ'.(sregs) ∗ gen_heap_interp σ'.(mem) ∗ strans_inv.
   Proof.
-    intros acc va pa ppn pc σ E Hacc Hallow Hcanon Hconcat Hmisa Hmenv Hhtif Hcp HSXL Heff Hss Hall HE.
+    intros acc va pa ppn pc σ E Hacc Hallow Hcanon Hconcat Hmisa Hmenv Hhtif Hcp HSXL Heff Hss Hall Hadm HE.
     iIntros "Hat Hri Hgh [(Hbit & Hb & Hstv) | (Hbit & Hk)]".
-    - iMod (bare_absorb acc va pa ppn pc σ E Hacc Hallow Hcanon Hconcat Hmisa Hmenv Hhtif Hcp HSXL Heff Hss Hall HE
+    - iMod (bare_absorb acc va pa ppn pc σ E Hacc Hallow Hcanon Hconcat Hmisa Hmenv Hhtif Hcp HSXL Heff Hss Hall Hadm HE
               with "Hat Hri Hgh Hb") as (σ') "(%Htr & %Hmdev & %Hsh & %Hpmp & Hri & Hgh & Hb)".
       iModIntro. iExists σ'.
       iSplit; [done |]. iSplit; [done |]. iSplit; [done |]. iSplit; [done |].
       iFrame "Hri Hgh". iLeft. iFrame "Hbit Hb Hstv".
     - iDestruct "Hk" as (root_ppn) "Ht".
-      iMod (res_absorb root_ppn acc va pa ppn pc σ E Hacc Hallow Hcanon Hconcat Hmisa Hmenv Hhtif Hcp HSXL Heff Hss Hall HE
+      iMod (res_absorb root_ppn acc va pa ppn pc σ E Hacc Hallow Hcanon Hconcat Hmisa Hmenv Hhtif Hcp HSXL Heff Hss Hall I HE
               with "Hat Hri Hgh Ht") as (σ') "(%Htr & %Hmdev & %Hsh & %Hpmp & Hri & Hgh & Ht)".
       iModIntro. iExists σ'.
       iSplit; [done |]. iSplit; [done |]. iSplit; [done |]. iSplit; [done |].
@@ -577,7 +578,8 @@ Section IntrDefs.
   Qed.
 
   Definition strans_regime : s_regime :=
-    SRegime strans_inv strans_absorb strans_transform.
+    SRegime strans_inv kadm_ident (fun _ _ H => H)
+            strans_absorb strans_transform.
 
   (* [sr_inv strans_regime] is definitionally [strans_inv] -- the bridge the
      leaf/engine call sites use without unfolding the record. *)
